Merge files

src/dafny/test.dfy
@@ -1,5 +1,20 @@
-include "Process.dfy"
-include "Endo.dfy"
+class Endokernel {
+    constructor() {}
+}
+
+class Process {
+    var endokernel: Endokernel;
+
+    constructor(endokernel:Endokernel)
+    {
+        this.endokernel := endokernel;
+    }
+
+    method exec() modifies this, endokernel {
+        // Uncommenting the following line can't eliminate the error on Line 25
+        // this.endokernel := new Endokernel();
+    }
+}
 
 class Test {
 
@@ -7,7 +22,9 @@ class Test {
         // Example of a simple execution of the Endokernel abstraction
         var endokernel:Endokernel := new Endokernel();
         var p:Process := new Process(endokernel);
-        p.exec();
+        p.exec(); // ERROR: call may violate context's modifies clause 
+                  //   Execution trace:
+                  //       (0,0): anon0
     }
 
     method Main()  {
